started update

SSA/Experimental/Bits/Fast/FiniteStateMachine.lean
@@ -1,12 +1,16 @@
 import Mathlib.Data.Fintype.Card
+import Mathlib.Data.FinEnum
 import Mathlib.Data.Fintype.Sum
 import Mathlib.Data.Fintype.Sigma
 import Mathlib.Data.Fintype.Pi
 import Mathlib.Data.Fintype.BigOperators
 import Mathlib.Tactic.Zify
 import Mathlib.Tactic.Ring
-import SSA.Experimental.Bits.Fast.Defs
+import SSA.Experimental.Bits.AutoStructs.Defs
+import SSA.Experimental.Bits.AutoStructs.FinEnum
 import SSA.Experimental.Bits.Fast.Circuit
+import SSA.Experimental.Bits.Fast.BitStream
+namespace AutoStructs
 
 open Sum
 
@@ -22,7 +26,7 @@ structure FSM (arity : Type) : Type 1 where
   The arity of the (finite) type `α` determines how many bits the internal carry state of this
   FSM has -/
   ( α  : Type )
-  [ i : Fintype α ]
+  [ i : FinEnum α ]
   [ dec_eq : DecidableEq α ]
   /--
   `initCarry` is the value of the initial internal carry state.
@@ -42,28 +46,7 @@ attribute [instance] FSM.i FSM.dec_eq
 
 namespace FSM
 
-variable {arity : Type} (p : FSM arity)
-
-instance : Std.Commutative Nat.add where
-  comm := fun a b => by simp only [Nat.add_eq]; omega
-
-instance : Std.Associative Nat.add where
-  assoc := fun a b => by simp only [Nat.add_eq]; omega
-
-/-- The size of the state space of the finite state machine. -/
-def stateSpaceSize : Nat := @Finset.univ p.α inferInstance |>.card
-
-
-/--
-Return the total size of the FSM as a function of all of its circuits.
-Note that this implicitly counts the size of the state space of the FSM,
-and consequently, is the natural notion of complexity of the FSM.
--/
-def circuitSize : Nat := Id.run do
-  let outCircSize := p.nextBitCirc none |>.size
-  let states := @Finset.univ p.α inferInstance
-  let stateCircSize := Finset.fold Nat.add  0 (fun a => p.nextBitCirc (.some a) |>.size) states
-  return outCircSize + stateCircSize
+variable {ar : Type} (p : FSM ar)
 
 /-- The state of FSM `p` is given by a function from `p.α` to `Bool`.
 
@@ -73,7 +56,7 @@ abbrev State : Type := p.α → Bool
 
 /-- `p.nextBit state in` computes both the next state bits and the output bit,
 where `state` are the *current* state bits, and `in` are the current input bits. -/
-def nextBit : p.State → (arity → Bool) → p.State × Bool :=
+def nextBit : p.State → (ar → Bool) → p.State × Bool :=
   fun carry inputBits =>
     let input := Sum.elim carry inputBits
     let newState : p.State  := fun (a : p.α) => (p.nextBitCirc (some a)).eval input
@@ -81,16 +64,41 @@ def nextBit : p.State → (arity → Bool) → p.State × Bool :=
     (newState, outBit)
 
 /-- `p.carry in i` computes the internal carry state at step `i`, given input *streams* `in` -/
-def carry (x : arity → BitStream) : ℕ → p.State
+def carry (x : ar → BitStream) : ℕ → p.State
   | 0 => p.initCarry
   | n+1 => (p.nextBit (carry x n) (fun i => x i n)).1
 
+lemma carry_eq_up_to :
+    (∀ ar k, k < n → x ar k = y ar k) →
+    p.carry x n = p.carry y n := by
+  induction n generalizing x y
+  case zero => intros; rfl
+  case succ n ih =>
+    rintro heq
+    simp [carry, @ih x y (by tauto)]
+    congr; simp_all only [lt_add_iff_pos_right, zero_lt_one]
+
+def carryBV (x : ar → BitVec w) : p.State :=
+  p.carry (fun ar => BitStream.ofBitVec (x ar)) w
+
 /-- `eval p` morally gives the function `BitStream → ... → BitStream` represented by FSM `p` -/
-def eval (x : arity → BitStream) : BitStream :=
+def eval (x : ar → BitStream) : BitStream :=
   fun n => (p.nextBit (p.carry x n) (fun i => x i n)).2
 
+lemma eval_eq_up_to :
+    (∀ ar k, k ≤ n → x ar k = y ar k) →
+    p.eval x n = p.eval y n := by
+  rintro h
+  simp [eval]
+  congr
+  apply carry_eq_up_to p (by rintro ar k hlt; apply h; omega)
+  ext; apply h; rfl
+
+def evalBV {w} (x : ar → BitVec w) : BitVec w :=
+  BitVec.ofFn fun k => p.eval (fun ar => BitStream.ofBitVec (x ar)) k
+
 /-- `eval'` is an alternative definition of `eval` -/
-def eval' (x : arity → BitStream) : BitStream :=
+def eval' (x : ar → BitStream) : BitStream :=
   BitStream.corec (fun ⟨x, (carry : p.State)⟩ =>
     let x_head  := (x · |>.head)
     let next    := p.nextBit carry x_head
@@ -99,11 +107,11 @@ def eval' (x : arity → BitStream) : BitStream :=
   ) (x, p.initCarry)
 
 /-- `p.changeInitCarry c` yields an FSM with `c` as the initial state -/
-def changeInitCarry (p : FSM arity) (c : p.α → Bool) : FSM arity :=
+def changeInitCarry (p : FSM ar) (c : p.α → Bool) : FSM ar :=
   { p with initCarry := c }
 
 theorem carry_changeInitCarry_succ
-    (p : FSM arity) (c : p.α → Bool) (x : arity → BitStream) : ∀ n,
+    (p : FSM ar) (c : p.α → Bool) (x : ar → BitStream) : ∀ n,
     (p.changeInitCarry c).carry x (n+1) =
       (p.changeInitCarry (p.nextBit c (fun a => x a 0)).1).carry
         (fun a i => x a (i+1)) n
@@ -113,7 +121,7 @@ theorem carry_changeInitCarry_succ
     simp [nextBit, carry, changeInitCarry]
 
 theorem eval_changeInitCarry_succ
-    (p : FSM arity) (c : p.α → Bool) (x : arity → BitStream) (n : ℕ) :
+    (p : FSM ar) (c : p.α → Bool) (x : ar → BitStream) (n : ℕ) :
     (p.changeInitCarry c).eval x (n+1) =
       (p.changeInitCarry (p.nextBit c (fun a => x a 0)).1).eval
         (fun a i => x a (i+1)) n := by
@@ -121,14 +129,13 @@ theorem eval_changeInitCarry_succ
   simp [eval, changeInitCarry, nextBit]
 
 /-- unfolds the definition of `eval` -/
-theorem eval_eq_carry (x : arity → BitStream) (n : ℕ) :
+theorem eval_eq_carry (x : ar → BitStream) (n : ℕ) :
     p.eval x n = (p.nextBit (p.carry x n) (fun i => x i n)).2 :=
   rfl
 
-
 /-- `p.changeVars f` changes the arity of an `FSM`.
 The function `f` determines how the new input bits map to the input expected by `p` -/
-def changeVars {arity2 : Type} (changeVars : arity → arity2) : FSM arity2 :=
+def changeVars {arity2 : Type} (changeVars : ar → arity2) : FSM arity2 :=
   { p with nextBitCirc := fun a => (p.nextBitCirc a).map (Sum.map id changeVars) }
 
 /--
@@ -137,13 +144,13 @@ a family of `n` FSMs `qᵢ` of posibly different arities `mᵢ`,
 and given yet another arity `m` such that `mᵢ ≤ m` for all `i`,
 we can compose `p` with `qᵢ` yielding a single FSM of arity `m`,
 such that each FSM `qᵢ` computes the `i`th bit that is fed to the FSM `p`. -/
-def compose [Fintype arity] [DecidableEq arity]
+def compose [FinEnum ar] [DecidableEq ar]
     (new_arity : Type)        -- `new_arity` is the resulting arity
-    (q_arity : arity → Type)  -- `q_arityₐ` is the arity of FSM `qₐ`
-    (vars : ∀ (a : arity), q_arity a → new_arity)
+    (q_arity : ar → Type)  -- `q_arityₐ` is the arity of FSM `qₐ`
+    (vars : ∀ (a : ar), q_arity a → new_arity)
     -- ^^ `vars` is the function that tells us, for each FSM `qₐ`,
     --     which bits of the final `new_arity` corresponds to the `q_arityₐ` bits expected by `qₐ`
-    (q : ∀ (a : arity), FSM (q_arity a)) : -- `q` gives the FSMs to be composed with `p`
+    (q : ∀ (a : ar), FSM (q_arity a)) : -- `q` gives the FSMs to be composed with `p`
     FSM new_arity :=
   { α := p.α ⊕ (Σ a, (q a).α),
     i := by letI := p.i; infer_instance,
@@ -171,11 +178,11 @@ def compose [Fintype arity] [DecidableEq arity]
               (fun a => inl (inr ⟨_, a⟩))
               (fun a => inr (vars x a))) }
 
-lemma carry_compose [Fintype arity] [DecidableEq arity]
+lemma carry_compose [FinEnum ar] [DecidableEq ar]
     (new_arity : Type)
-    (q_arity : arity → Type)
-    (vars : ∀ (a : arity), q_arity a → new_arity)
-    (q : ∀ (a : arity), FSM (q_arity a))
+    (q_arity : ar → Type)
+    (vars : ∀ (a : ar), q_arity a → new_arity)
+    (q : ∀ (a : ar), FSM (q_arity a))
     (x : new_arity → BitStream) : ∀ (n : ℕ),
     (p.compose new_arity q_arity vars q).carry x n =
       let z := p.carry (λ a => (q a).eval (fun i => x (vars _ i))) n
@@ -204,11 +211,11 @@ lemma carry_compose [Fintype arity] [DecidableEq arity]
         · simp
 
 /-- Evaluating a composed fsm is equivalent to composing the evaluations of the constituent FSMs -/
-lemma eval_compose [Fintype arity] [DecidableEq arity]
+lemma eval_compose [FinEnum ar] [DecidableEq ar]
     (new_arity : Type)
-    (q_arity : arity → Type)
-    (vars : ∀ (a : arity), q_arity a → new_arity)
-    (q : ∀ (a : arity), FSM (q_arity a))
+    (q_arity : ar → Type)
+    (vars : ∀ (a : ar), q_arity a → new_arity)
+    (q : ∀ (a : ar), FSM (q_arity a))
     (x : new_arity → BitStream) :
     (p.compose new_arity q_arity vars q).eval x =
       p.eval (λ a => (q a).eval (fun i => x (vars _ i))) := by
@@ -230,7 +237,8 @@ def and : FSM Bool :=
   { α := Empty,
     initCarry := Empty.elim,
     nextBitCirc := fun a => a.elim
-      ((Circuit.var true (inr true)) &&&
+      (Circuit.and
+        (Circuit.var true (inr true))
         (Circuit.var true (inr false))) Empty.elim }
 
 @[simp] lemma eval_and (x : Bool → BitStream) : and.eval x = (x true) &&& (x false) := by
@@ -240,159 +248,23 @@ def or : FSM Bool :=
   { α := Empty,
     initCarry := Empty.elim,
     nextBitCirc := fun a => a.elim
-      ((Circuit.var true (inr true)) |||
+      (Circuit.or
+        (Circuit.var true (inr true))
         (Circuit.var true (inr false))) Empty.elim }
 
 @[simp] lemma eval_or (x : Bool → BitStream) : or.eval x = (x true) ||| (x false) := by
-  ext n; cases n <;> simp [and, eval, nextBit]
+  ext n; cases n <;> simp [or, eval, nextBit]
 
 def xor : FSM Bool :=
   { α := Empty,
     initCarry := Empty.elim,
     nextBitCirc := fun a => a.elim
-      ( (Circuit.var true (inr true)) ^^^
+      (Circuit.xor
+        (Circuit.var true (inr true))
         (Circuit.var true (inr false))) Empty.elim }
 
-/-- Equality, or alternatively, negation of the xor -/
-def nxor : FSM Bool :=
-  { α := Empty,
-    initCarry := Empty.elim,
-    nextBitCirc := fun a =>
-     match a with
-     | none =>
-      -- x ⊕ y ⊕ T
-      -- 0 ⊕ 0 ⊕ 1 = 1
-      -- 0 ⊕ 1 ⊕ 1 = 0 -- value is 0 iff they differ
-      -- 1 ⊕ 0 ⊕ 1 = 0 -- value is 1 iff they differ.
-      -- 1 ⊕ 1 ⊕ 1 = 1
-      (Circuit.tru ^^^
-        ( (Circuit.var true (inr true)) ^^^
-        (Circuit.var true (inr false))))
-     | some empty => empty.elim
-  }
-
-def simplify (p : FSM arity) : FSM arity := {
-  α := p.α
-  initCarry := p.initCarry
-  -- nextBitCirc := Circuit.simplify ∘ p.nextBitCirc
-  nextBitCirc := p.nextBitCirc
-}
-
-/-- Evaluating the value after `simplify` is the same as the original value. -/
-@[simp] lemma eval_simplify :
-    p.simplify.eval = p.eval := rfl
-
-
-/--
-Scan a sequence of booleans with the bitwise and operator
-Thus:
-
-```lean
-(scanAnd)[0] = in[0] &&& True
-(scanAnd)[1] = in[1] &&& scanAnd[0]
-(scanAnd)[2] = in[2] &&& scanAnd[1]
-```
--/
-def scanAnd  : FSM Unit :=
-  {
-   α := Unit,
-   initCarry := fun () => true,
-   nextBitCirc := fun _a => (Circuit.var true (inl ())) &&& (Circuit.var true (inr ()))
-  }
-
-@[simp]
-lemma eval_scanAnd_zero (x : Unit → BitStream) : scanAnd.eval x 0 = (x () 0) := by
-  simp[eval, nextBit, scanAnd, and, carry]
-
-@[simp]
-lemma eval_scanAnd_succ (x : Unit → BitStream) (n : Nat) :
-    (scanAnd.eval x (n+1)) = ((scanAnd.eval x n) && (x () (n+1)))  := by
-  simp [eval, nextBit, scanAnd, and, carry]
-
-/-- The result of `scanAnd` is true at `n` iff the bitvector has been true upto (and including) `n`. -/
-@[simp] lemma eval_scanAnd_true_iff (x : Unit → BitStream) (n : Nat) : scanAnd.eval x n = true ↔ (∀ (i : Nat), (hi : i ≤ n) → x () i = true) := by
-  induction n
-  case zero => simp [eval, nextBit, scanAnd, and, carry]
-  case succ n ih =>
-    rw [eval_scanAnd_succ]
-    constructor
-    · intros h
-      intros i hi
-      have hScan := Bool.and_elim_left h
-      have hxn := Bool.and_elim_right h
-      have hi : (i = n+1) ∨ (i < n + 1) := by omega
-      rcases hi with rfl | hi
-      · exact hxn
-      · apply ih.mp
-        · exact hScan
-        · omega
-    · intros h
-      have := h (n + 1) (by omega)
-      simp [this]
-      apply ih.mpr
-      intros j hj
-      exact h j (by omega)
-
 @[simp] lemma eval_xor (x : Bool → BitStream) : xor.eval x = (x true) ^^^ (x false) := by
-  ext n; cases n <;> simp [and, eval, nextBit]
-
-@[simp] lemma eval_nxor (x : Bool → BitStream) : nxor.eval x = ((x true).nxor (x false)) := by
-  ext n; cases n
-  · simp [nxor, eval, nextBit]
-  · simp [nxor, eval, nextBit]
-
-def scanOr  : FSM Unit :=
-  {
-   α := Unit,
-   initCarry := fun () => false,
-   nextBitCirc := fun _α => (Circuit.var true (inl ())) ||| (Circuit.var true (inr ()))
-  }
-
-@[simp]
-lemma eval_scanOr_zero (x : Unit → BitStream) : scanOr.eval x 0 = (x () 0) := by
-  simp[eval, nextBit, scanOr, and, carry]
-
-@[simp]
-lemma eval_scanOr_succ (x : Unit → BitStream) (n : Nat) :
-    (scanOr.eval x (n+1)) = ((scanOr.eval x n) || (x () (n+1)))  := by
-  simp [eval, nextBit, scanOr, and, carry]
-
-/-- The result of `scanOr` is false at `n` iff the bitvector has been false upto (and including) time `n`. -/
-@[simp] lemma eval_scanor_false_iff (x : Unit → BitStream) (n : Nat) : scanOr.eval x n = false ↔ (∀ (i : Nat), (hi : i ≤ n) → x () i = false) := by
-  induction n
-  case zero => simp [eval, nextBit, scanOr, and, carry]
-  case succ n ih =>
-    rw [eval_scanOr_succ]
-    constructor
-    · intros h
-      intros i hi
-      have := Bool.or_eq_false_iff.mp h
-      have hi : (i = n+1) ∨ (i < n + 1) := by omega
-      rcases hi with rfl | hi
-      · simp [this]
-      · apply ih.mp
-        · simp [this]
-        · omega
-    · intros h
-      have := h (n + 1) (by omega)
-      simp [this]
-      apply ih.mpr
-      intros j hj
-      exact h j (by omega)
-
-/-- Show that the FSM and the bitstream computations agree for `scanOr`. -/
-@[simp] lemma eval_scanOr (x : Unit → BitStream) : scanOr.eval x = (x ()).scanOr := by
-  ext n;
-  induction n
-  case zero => simp
-  case succ n ih => simp [ih]
-
-/-- Show that the FSM and the bitstream computations agree for `scanOr`. -/
-@[simp] lemma eval_scanAnd (x : Unit → BitStream) : scanAnd.eval x = (x ()).scanAnd := by
-  ext n;
-  induction n
-  case zero => simp
-  case succ n ih => simp [ih]
+  ext n; cases n <;> simp [xor, eval, nextBit]
 
 def add : FSM Bool :=
   { α := Unit,
@@ -418,9 +290,11 @@ theorem carry_add_succ (x : Bool → BitStream) (n : ℕ) :
     simp [carry, BitStream.addAux, nextBit, add, BitVec.adcb]
   | succ n ih =>
     unfold carry
-    simp [nextBit, ih, Circuit.eval, BitStream.addAux, BitVec.adcb]
+    simp [nextBit, ih, Circuit.eval, BitStream.addAux, BitVec.adcb, nextBitCirc, Sum.elim]
+    sorry -- TODO: fix this proof
 
-@[simp] theorem carry_zero (x : arity → BitStream) : carry p x 0 = p.initCarry := rfl
+
+@[simp] theorem carry_zero (x : ar → BitStream) : carry p x 0 = p.initCarry := rfl
 @[simp] theorem initCarry_add : add.initCarry = (fun _ => false) := rfl
 
 @[simp] lemma eval_add (x : Bool → BitStream) : add.eval x = (x true) + (x false) := by
@@ -451,7 +325,7 @@ def sub : FSM Bool :=
 theorem carry_sub (x : Bool → BitStream) : ∀ (n : ℕ), sub.carry x (n+1) =
     fun _ => (BitStream.subAux (x true) (x false) n).2
   | 0 => by
-    simp [carry, nextBit, funext_iff, BitStream.subAux, sub]
+    simp [carry, nextBit, BitStream.subAux, sub]
   | n+1 => by
     rw [carry, carry_sub _ n]
     simp [nextBit, eval, sub, BitStream.sub, BitStream.subAux, Bool.xor_not_left']
@@ -465,41 +339,6 @@ theorem eval_sub (x : Bool → BitStream) : sub.eval x = (x true) - (x false) :=
   · rw [eval, carry_sub]
     simp [nextBit, eval, sub, BitStream.sub, BitStream.subAux]
 
-/-!
-We define a borrow automata, whose output stream is the internal state of the subtraction automata,
-which is the bits to be borrowed.
-
-Compare against subAux.2
--/
-
-def borrow : FSM Bool :=
-  { α := Unit,
-    -- Internal state is the current borrow.
-    initCarry := fun _ => false,
-    -- | TODO: check that this is in fact the borrow bit of the subtraction automata.
-    -- Check that we do correctly compute the borrow bit here.
-    nextBitCirc := fun _i =>
-      let borrow := Circuit.var true (inl ())
-      let a := Circuit.var true (inr true)
-      let nota := Circuit.var false (inr true)
-      let b := Circuit.var true (inr false)
-      -- let borrow := (subAux x y n).2
-      -- computing x - y:
-      -- x y b | out-borrow
-      -- 0 0 0 | 0
-      -- 0 0 1 | 1
-      -- 0 1 0 | 1
-      -- 0 1 1 | 1
-      -- 1 0 0 | 0
-      -- 1 0 1 | 0
-      -- 1 1 0 | 0
-      -- 1 1 1 | 1
-      -- (!a && b || ((!(xor a b)) && borrow))
-      (nota &&& b/- !a && b-/) |||
-      ((~~~ (a ^^^ b) /- !(xor a b) -/) &&& borrow)
-
-  }
-
 def neg : FSM Unit :=
   { α := Unit,
     i := by infer_instance,
@@ -512,7 +351,7 @@ def neg : FSM Unit :=
 theorem carry_neg (x : Unit → BitStream) : ∀ (n : ℕ), neg.carry x (n+1) =
     fun _ => (BitStream.negAux (x ()) n).2
   | 0 => by
-    simp [carry, nextBit, funext_iff, BitStream.negAux, neg]
+    simp [carry, nextBit, BitStream.negAux, neg]
   | n+1 => by
     rw [carry, carry_neg _ n]
     simp [nextBit, eval, neg, BitStream.neg, BitStream.negAux, Bool.xor_not_left']
@@ -558,7 +397,7 @@ def one : FSM (Fin 0) :=
   ext n
   cases n
   · rfl
-  · simp [eval, carry_one, nextBit]
+  · simp! [eval, carry_one, nextBit, one, mk]
 
 def negOne : FSM (Fin 0) :=
   { α := Empty,
@@ -569,10 +408,7 @@ def negOne : FSM (Fin 0) :=
 @[simp] lemma eval_negOne (x : Fin 0 → BitStream) : negOne.eval x = BitStream.negOne := by
   ext; simp [negOne, eval, nextBit]
 
-/--
-An FSM whose first output is `b`, and later outputs are whatever the input is.
--/
-def ls (b : Bool) : FSM Unit :=
+@[simp] def ls (b : Bool) : FSM Unit :=
   { α := Unit,
     initCarry := fun _ => b,
     nextBitCirc := fun x =>
@@ -583,7 +419,7 @@ def ls (b : Bool) : FSM Unit :=
 theorem carry_ls (b : Bool) (x : Unit → BitStream) : ∀ (n : ℕ),
     (ls b).carry x (n+1) = fun _ => x () n
   | 0 => by
-    simp [carry, nextBit, funext_iff, ls]
+    simp [carry, nextBit, ls]
   | n+1 => by
     rw [carry, carry_ls _ _ n]
     simp [nextBit, eval, ls]
@@ -593,7 +429,7 @@ theorem carry_ls (b : Bool) (x : Unit → BitStream) : ∀ (n : ℕ),
   ext n
   cases n
   · rfl
-  · simp [carry_ls, eval, nextBit, BitStream.concat]
+  · simp [ls, carry, carry_ls, eval, nextBit, BitStream.concat]
 
 def var (n : ℕ) : FSM (Fin (n+1)) :=
   { α := Empty,
@@ -615,7 +451,7 @@ def incr : FSM Unit :=
 theorem carry_incr (x : Unit → BitStream) : ∀ (n : ℕ),
     incr.carry x (n+1) = fun _ => (BitStream.incrAux (x ()) n).2
   | 0 => by
-    simp [carry, nextBit, funext_iff, BitStream.incrAux, incr]
+    simp [carry, nextBit, BitStream.incrAux, incr]
   | n+1 => by
     rw [carry, carry_incr _ n]
     simp [nextBit, eval, incr, incr, BitStream.incrAux]
@@ -638,7 +474,7 @@ def decr : FSM Unit :=
 theorem carry_decr (x : Unit → BitStream) : ∀ (n : ℕ), decr.carry x (n+1) =
     fun _ => (BitStream.decrAux (x ()) n).2
   | 0 => by
-    simp [carry, nextBit, funext_iff, BitStream.decrAux, decr]
+    simp [carry, nextBit, BitStream.decrAux, decr]
   | n+1 => by
     rw [carry, carry_decr _ n]
     simp [nextBit, eval, decr, BitStream.decrAux]
@@ -677,100 +513,66 @@ def repeatBit : FSM Unit where
   nextBitCirc := fun _ =>
     .or (.var true <| .inl ()) (.var true <| .inr ())
 
--- @[simp] theorem eval_repeatBit :
---     repeatBit.eval x = BitStream.repeatBit (x ()) := by
---   unfold BitStream.repeatBit
---   rw [eval_eq_eval', eval']
---   apply BitStream.corec_eq_corec
---     (R := fun a b => a.1 () = b.2 ∧ (a.2 ()) = b.1)
---   · simp [repeatBit]
---   · intro ⟨y, a⟩ ⟨b, x⟩ h
---     simp at h
---     simp [h, nextBit, BitStream.head]
-
 end FSM
 
-/-- An `FSMTermSolution `t` is an FSM with a witness that the FSM evaluates to the same value as `t` does -/
-structure FSMTermSolution (t : Term) extends FSM (Fin t.arity) where
-  ( good : t.evalFin = toFSM.eval )
+structure FSMSolution (t : Term) extends FSM (Fin t.arity) where
+  ( good : t.evalFinStream = toFSM.eval )
 
-
-/-- Compose two automata together, where `q` is an FSM -/
-def composeUnaryAux
-    (p : FSM Unit)
-    (q : FSM arity) :
-    FSM arity :=
-  p.compose
-    arity
-    _
-    (λ _ => id)
-    (λ _ => q)
-
-/-- Compose two automata together, where `q` is an FSMTermSolution -/
 def composeUnary
     (p : FSM Unit)
     {t : Term}
-    (q : FSMTermSolution t) :
-    FSM (Fin t.arity) := composeUnaryAux p q.toFSM
+    (q : FSMSolution t) :
+    FSM (Fin t.arity) :=
+  p.compose
+    (Fin t.arity)
+    _
+    (λ _ => id)
+    (λ _ => q.toFSM)
 
-def composeBinaryAux
+def composeBinary
     (p : FSM Bool)
-    (q₁ : FSM (Fin a₁))
-    (q₂ : FSM (Fin a₂)) :
-    FSM (Fin (max a₁ a₂)) :=
-  p.compose (Fin (max a₁ a₂))
-    (λ b => Fin (cond b a₁ a₂))
+    {t₁ t₂ : Term}
+    (q₁ : FSMSolution t₁)
+    (q₂ : FSMSolution t₂) :
+    FSM (Fin (max t₁.arity t₂.arity)) :=
+  p.compose (Fin (max t₁.arity t₂.arity))
+    (λ b => Fin (cond b t₁.arity t₂.arity))
+    (λ b i => Fin.castLE (by cases b <;> simp) i)
+    (λ b => match b with
+      | true => q₁.toFSM
+      | false => q₂.toFSM)
+
+def composeBinary'
+    (p : FSM Bool)
+    {n m : Nat}
+    (q₁ : FSM (Fin n))
+    (q₂ : FSM (Fin m)) :
+    FSM (Fin (max n m)) :=
+  p.compose (Fin (max n m))
+    (λ b => Fin (cond b n m))
     (λ b i => Fin.castLE (by cases b <;> simp) i)
     (λ b => match b with
       | true => q₁
       | false => q₂)
 
-/-- Compose two binary opeators -/
-def composeBinary
-    (p : FSM Bool)
-    {t₁ t₂ : Term}
-    (q₁ : FSMTermSolution t₁)
-    (q₂ : FSMTermSolution t₂) :
-    FSM (Fin (max t₁.arity t₂.arity)) := composeBinaryAux p q₁.toFSM q₂.toFSM
-
-
-@[simp] lemma composeUnaryAux_eval
-    (p : FSM Unit)
-    (q : FSM arity)
-    (x : arity → BitStream) :
-    (composeUnaryAux p q).eval x = p.eval (λ _ => q.eval x) := by
-  simp [composeUnaryAux, FSM.eval_compose]
-
 @[simp] lemma composeUnary_eval
     (p : FSM Unit)
     {t : Term}
-    (q : FSMTermSolution t)
+    (q : FSMSolution t)
     (x : Fin t.arity → BitStream) :
-    (composeUnary p q).eval x = p.eval (λ _ => t.evalFin x) := by
-  simp [composeUnary, FSM.eval_compose, q.good]
-
-@[simp] lemma composeBinaryAux_eval
-    (p : FSM Bool)
-    (q₁ : FSM (Fin a₁))
-    (q₂ : FSM (Fin a₂))
-    (x : Fin (max a₁ a₂) → BitStream) :
-    (composeBinaryAux p q₁ q₂).eval x = p.eval
-      (λ b => cond b (q₁.eval (fun i => x (Fin.castLE (by simp) i)))
-                  (q₂.eval (fun i => x (Fin.castLE (by simp) i)))) := by
-  rw [composeBinaryAux, FSM.eval_compose]
-  ext b
-  cases b <;> dsimp <;> congr <;> funext b <;> cases b <;> simp
+    (composeUnary p q).eval x = p.eval (λ _ => t.evalFinStream x) := by
+  rw [composeUnary, FSM.eval_compose, q.good]; rfl
 
 @[simp] lemma composeBinary_eval
     (p : FSM Bool)
     {t₁ t₂ : Term}
-    (q₁ : FSMTermSolution t₁)
-    (q₂ : FSMTermSolution t₂)
+    (q₁ : FSMSolution t₁)
+    (q₂ : FSMSolution t₂)
     (x : Fin (max t₁.arity t₂.arity) → BitStream) :
     (composeBinary p q₁ q₂).eval x = p.eval
-      (λ b => cond b (t₁.evalFin (fun i => x (Fin.castLE (by simp) i)))
-                  (t₂.evalFin (fun i => x (Fin.castLE (by simp) i)))) := by
-  rw [composeBinary, composeBinaryAux, FSM.eval_compose, q₁.good, q₂.good]
+      (λ b => cond b (t₁.evalFinStream (fun i => x (Fin.castLE (by simp) i)))
+                  (t₂.evalFinStream (fun i => x (Fin.castLE (by simp) i)))) := by
+  rw [composeBinary, FSM.eval_compose, q₁.good, q₂.good]
   ext b
   cases b <;> dsimp <;> congr <;> funext b <;> cases b <;> simp
 
@@ -778,294 +580,9 @@ instance {α β : Type} [Fintype α] [Fintype β] (b : Bool) :
     Fintype (cond b α β) := by
   cases b <;> simp <;> infer_instance
 
-
-namespace FSM
-
-/--
-A finite state machine whose outputs are the bits of the natural number `n`,
-in least to most significant bit order.
-
-See that this uses only as much as as *log₂ n*, which is the correct
-number of bits necessary to count up to `n`.
--/
-def ofNat (n : Nat)  : FSM (Fin 0) :=
-  match hn : n with
-  | 0 => FSM.zero
-  | n' + 1 =>
-    let bit := n.testBit 0
-    let m := n / 2
-    have h : m < n := by
-      simp [m];
-      apply Nat.div_lt_iff_lt_mul _ |>.mpr
-      · omega
-      · decide
-    composeUnaryAux (FSM.ls bit) (ofNat m)
-
-@[simp]
-theorem ofNat_zero : ofNat 0 = FSM.zero :=
-  by simp [ofNat]
-
-/-- Evaluating 'const n' gives us the bits of the value of 'const n'.-/
-@[simp]
-theorem eval_ofNat (n : Nat) (i : Nat) {env : Fin 0 → BitStream} :
-    (ofNat n).eval env i = n.testBit i := by
-  induction n using Nat.div2Induction generalizing i
-  case ind n hn =>
-    rcases n with rfl | hn
-    case zero => simp
-    case succ n =>
-      simp [ofNat]
-      have : n + 1 > 0 := by omega
-      specialize (hn this)
-      cases i
-      · case zero => simp
-      · case succ i' =>
-        simp [hn, Nat.testBit_succ]
-
-
-/-- Test the 'k'th bit of an integer.
-
-* negSucc:
-   - (n + 1)
-   = -n - 1
-   = (!x + 1) - 1 = !x
--/
-def _root_.Int.testBit' (i : Int) (k : Nat) : Bool :=
-  match i with 
-  | .ofNat n => n.testBit k
-  | .negSucc n => !(n.testBit k)
-
-/--
-the 'k'th bit of 'w' is equal to the 'k'th bit we get by testing the integer representation.
--/
-theorem BitVec.getLsbD_eq_toInt_testBit' (b : BitVec w) (hk : k < w) : b.getLsbD k = b.toInt.testBit' k := by
-  rw [BitVec.getLsbD]
-  rw [BitVec.toInt_eq_toNat_cond]
-  by_cases hb : 2 * b.toNat < 2^w
-  · simp [hb]
-    rw [Int.testBit'.eq_def]
-  · simp [hb]
-    have : ↑b.toNat - 2 ^ w = Int.subNatNat b.toNat (2 ^ w) := by norm_cast
-    rw [Int.testBit'.eq_def, this, Int.subNatNat_of_lt (by omega)]
-    simp
-    let notb := (~~~ b).toNat
-    rw [show 2^w - b.toNat - 1 = 2^w - 1 - b.toNat by omega, ← BitVec.toNat_not]
-    rw [← BitVec.getLsbD, ← BitVec.getLsbD]
-    simp
-    omega
-
-
-/--
-If `i < -1`, then `i` is less than `i / 2`.
-If `i = -1`, then `-1 / 2 = -1` (floor division of integers).
--/
-private theorem Int.lt_of_neg {i : Int} (hi : i < - 1) : i < i / 2 := by
-  have h : (2 ∣ i) ∨ (2 ∣ (i - 1)) := by
-    omega
-  rcases h with h | h
-  · rw [Int.div_def]
-    apply Int.lt_ediv_of_mul_lt <;> omega
-  · have hi : i = (i - 1) + 1 := by omega
-    conv =>
-      rhs
-      rw [hi]
-    rw [Int.add_ediv_of_dvd_left]
-    · simp only [Int.reduceDiv, add_zero]
-      apply Int.lt_ediv_of_mul_lt
-      · omega
-      · exact h
-      · omega
-    · omega
-
-/--
-Show how to build a bitvector representation from a `negSucc`.
-The theory of `Int.testBit` tells us that we can get the bits from `!(n.testBit k)`.
--/
-def ofNegInt (i : Int) (hi : i < 0) : FSM (Fin 0) :=
-  if hi' : i = -1 then  
-    FSM.negOne
-  else
-    let bit := i.testBit' 0
-    let m := i / 2
-    let k := ofNegInt m (by omega)
-    composeUnaryAux (FSM.ls bit) k
-  termination_by (-i |>.toNat)
-  decreasing_by
-    simp [hi]
-    apply Int.lt_of_neg
-    omega
-
-/-- 
--/
-@[simp] theorem eval_ofNegInt (x : Int) (hx : x < 0)  (i : Nat) {env : Fin 0 → BitStream} :
-    (ofNegInt x hx).eval env i = BitStream.ofInt x i := by
-  rcases x with x | x 
-  · simp at hx; omega
-  · simp [BitStream.ofInt]
-    induction x
-    case zero => 
-      simp [ofNegInt]
-    case succ x ih =>
-      rw [ofNegInt]
-      have hi' : Int.negSucc (x + 1) ≠ -1 := by omega
-      simp [hi']
-      simp [BitStream.concat]
-      sorry
-
-/-- Build a finite state machine for the integer `i` -/
-def ofInt (x : Int) : FSM (Fin 0) := 
-  if hi : x ≥ 0 then
-    ofNat x.toNat
-  else
-    ofNegInt x (by omega)
-
-/-- 
-The result of `FSM.ofInt x` matches with `BitStream.ofInt x`.
--/
-theorem eval_ofInt (x : Int) (i : Nat) {env : Fin 0 → BitStream} :
-    (ofInt x).eval env i = BitStream.ofInt x i := by
-  rcases x with x | x
-  · simp [ofInt, BitStream.ofInt]
-  · simp [ofInt, BitStream.ofInt]
-
-
-/-- Identity finite state machine -/
-def id : FSM Unit := {
- α := Empty,
- initCarry := Empty.elim,
- nextBitCirc := fun a => 
-   match a with
-   | none => (Circuit.var true (inr ()))
-   | some f => f.elim
-}
-
-/-- Build logical shift left automata by `n` bits -/
-def shiftLeft (n : Nat) : FSM Unit :=
-  match n with
-  | 0 => FSM.id
-  | n + 1 => composeUnaryAux (FSM.ls false) (shiftLeft n)
-
-/--
-Build an FSM whose state is `true` at step `n`,
-and `false` everywhere else.
--/
-def trueOnlyAt (n : Nat) : FSM (Fin 0) := ofNat (1 <<< n)
-
-/- `Nat.testBit 1 i = false` if and only if `i` is nonzero. -/
-@[simp]
-private theorem _root_.Nat.testBit_one_eq_false_iff (i : Nat) :
-    Nat.testBit 1 i = false ↔ i ≠ 0 := by
-  constructor
-  · simp only [ne_eq]
-    by_cases hi : i = 0 <;> simp [hi]
-  · intros h
-    rw [Nat.testBit, Nat.shiftRight_eq_div_pow]
-    have : 2^i ≥ 2 := by
-      exact Nat.le_self_pow h 2
-    simp only [Nat.one_and_eq_mod_two, Nat.mod_two_bne_zero, beq_eq_false_iff_ne,
-      ne_eq, Nat.mod_two_not_eq_one]
-    rw [Nat.mod_eq_of_lt]
-    · apply Nat.div_eq_zero_iff |>.mpr; omega
-    · apply Nat.div_lt_of_lt_mul
-      omega
-
-/--
-`falseOnlyAt n` builds an FSM that is `false` at state `n` and
-`true` everywhere else. This is useful to build a predicate that
-checks if we are in the `n`th state.
--/
-@[simp]
-theorem eval_trueOnlyAt (n : Nat) (i : Nat) {env : Fin 0 → BitStream} :
-    (trueOnlyAt n).eval env i = decide (i = n) := by
-  simp [trueOnlyAt]
-  by_cases hn : i = n
-  · simp [hn]
-  · simp [hn]
-    omega
-
-/--
-Build an FSM whose state is `false` at step `n`,
-and `true` everywhere else.
--/
-def falseOnlyAt (n : Nat) : FSM (Fin 0) :=
-  composeUnaryAux FSM.not (trueOnlyAt n)
-
-/--
-`falseOnlyAt n` builds an FSM that is `false` at state `n` and
-`true` everywhere else. This is useful to build a predicate that
-checks if we are in the `n`th state.
--/
-@[simp] theorem eval_falseOnlyAt (n : Nat) (i : Nat) {env : Fin 0 → BitStream} :
-    (falseOnlyAt n).eval env i = !decide (i = n) := by simp [falseOnlyAt]
-
-/--
-Build an FSM whose value is 'true' for states [0, 1, ... n),
-and 'false' after.
--/
-def trueUptoExcluding (n : Nat) : FSM (Fin 0) :=
-  ofNat (BitVec.allOnes n).toNat
-@[simp] theorem eval_trueUptoExcluding (n : Nat) (i : Nat) {env : Fin 0 → BitStream} :
-    (trueUptoExcluding n).eval env i = decide (i < n) := by simp [trueUptoExcluding]
-
-def falseAfterIncluding (n : Nat) : FSM (Fin 0) := trueUptoExcluding n
-private theorem falseAfterIncluding_false_iff (n i : Nat) {env : Fin 0 → BitStream} :
-  (falseAfterIncluding n).eval env i = false ↔ i ≥ n := by simp [falseAfterIncluding];
-
-/--
-Build an FSM whose value is 'true' for states [0, 1, ... n] (including the endpoint),
-and 'false' after.
--/
-def trueUptoIncluding (n : Nat) : FSM (Fin 0) := ofNat (BitVec.allOnes (n+1)).toNat
-@[simp] theorem eval_trueUptoIncluding (n : Nat) (i : Nat) {env : Fin 0 → BitStream} :
-    (trueUptoIncluding n).eval env i = decide (i ≤ n) := by
-  simp [trueUptoIncluding]; omega
-def falseAfterExcluding (n : Nat) : FSM (Fin 0) := trueUptoIncluding n
-private theorem falseAfterExcluding_false_iff (n i : Nat) {env : Fin 0 → BitStream} :
-  (falseAfterExcluding n).eval env i = false ↔ i > n := by simp [falseAfterExcluding]
-
-/--
-Build an FSM whose value is and 'false' for the first [0, 1, ... n), and 'true' for [n, n + 1, ...).
--/
-def falseUptoExcluding (n : Nat) : FSM (Fin 0) := composeUnaryAux FSM.not (FSM.trueUptoExcluding n)
-@[simp] theorem eval_falseUptoExcluding (n : Nat) (i : Nat) {env : Fin 0 → BitStream} :
-    (falseUptoExcluding n).eval env i = decide (n ≤ i) := by
-  simp [falseUptoExcluding];
-  by_cases hi : i < n <;> (simp [hi]; try omega)
-/--
-Psychological theorem to see that 'i < n'
-if and only if 'falseUptoExcluding' evaluates to 'false
--/
-private theorem falseUptoExcluding_eq_false_iff (n : Nat) (i : Nat) {env : Fin 0 → BitStream} :
-    ((falseUptoExcluding n).eval env i = false) ↔ i < n := by simp;
-
-/--
-Build an FSM whose value is false' for the first [0, 1, ... n],
-and 'true' for (n, n + 1, ...) (excluding the startpoint)
--/
-def falseUptoIncluding (n : Nat) : FSM (Fin 0) :=
-  composeUnaryAux FSM.not (FSM.trueUptoIncluding n)
-@[simp] theorem eval_falseUptoIncluding (n : Nat) (i : Nat) {env : Fin 0 → BitStream} :
-    (falseUptoIncluding n).eval env i = decide (n < i) := by
-  simp [falseUptoIncluding];
-  by_cases hi : n < i <;> (simp [hi]; try omega)
-/--
-Psychological theorem to see that 'i ≤ n'
-if and only if 'falseUptoExcluding' evaluates to 'false
--/
-private theorem falseUptoIncluding_eq_false_iff (n : Nat) (i : Nat) {env : Fin 0 → BitStream} :
-    ((falseUptoIncluding n).eval env i = false) ↔ i ≤ n := by simp
-
-end FSM
-
 open Term
 
-/--
-Note that **this is the value that is run by decide**.
--/
-def termEvalEqFSM : ∀ (t : Term), FSMTermSolution t
-  | ofNat n =>
-    { toFSM := FSM.ofNat n,
-      good := by ext; simp [Term.evalFin] }
+def termEvalEqFSM : ∀ (t : Term), FSMSolution t
   | var n =>
     { toFSM := FSM.var n,
       good := by ext; simp [Term.evalFin] }
@@ -1093,10 +610,6 @@ def termEvalEqFSM : ∀ (t : Term), FSMTermSolution t
     let q₂ := termEvalEqFSM t₂
     { toFSM := composeBinary FSM.xor q₁ q₂,
       good := by ext; simp }
-  | ls b t =>
-    let q := termEvalEqFSM t
-    { toFSM := by dsimp [arity]; exact composeUnary (FSM.ls b) q,
-      good := by ext; simp }
   | Term.not t =>
     let q := termEvalEqFSM t
     { toFSM := by dsimp [arity]; exact composeUnary FSM.not q,
@@ -1115,297 +628,7 @@ def termEvalEqFSM : ∀ (t : Term), FSMTermSolution t
     let q := termEvalEqFSM t
     { toFSM := by dsimp [arity]; exact composeUnary FSM.neg q,
       good := by ext; simp }
-  | incr t =>
-    let q := termEvalEqFSM t
-    { toFSM := by dsimp [arity]; exact composeUnary FSM.incr q,
-      good := by ext; simp }
-  | decr t =>
-    let q := termEvalEqFSM t
-    { toFSM := by dsimp [arity]; exact composeUnary FSM.decr q,
-      good := by ext; simp }
-  | shiftL t k =>
-     let q := termEvalEqFSM t
-     {
-       toFSM := by dsimp [arity]; exact composeUnary (FSM.shiftLeft k) q,
-       good := by ext; simp; sorry
-     }
-  -- | repeatBit t =>
-  --   let p := termEvalEqFSM t
-  --   { toFSM := by dsimp [arity]; exact composeUnary FSM.repeatBit p,
-  --     good := by ext; simp }
 
-/-!
-FSM that implement bitwise-and. Since we use `0` as the good state,
-we keep the invariant that if both inputs are good and our state is `0`, then we produce a `0`.
-If not, we produce an infinite sequence of `1`.
--/
-def and : FSM Bool :=
-  { α := Unit,
-    initCarry := fun _ => false,
-    nextBitCirc := fun a =>
-      match a with
-      | some () =>
-             -- Only if both are `0` we produce a `0`.
-             (Circuit.var true (inr false)  |||
-             ((Circuit.var false (inr true) |||
-              -- But if we have failed and have value `1`, then we produce a `1` from our state.
-              (Circuit.var true (inl ())))))
-      | none => -- must succeed in both arguments, so we are `0` if both are `0`.
-                Circuit.var true (inr true) |||
-                Circuit.var true (inr false)
-                }
-
-/-!
-FSM that implement bitwise-or. Since we use `0` as the good state,
-we keep the invariant that if either inputs is `0` then our state is `0`.
-If not, we produce a `1`.
--/
-def or : FSM Bool :=
-  { α := Unit,
-    initCarry := fun _ => false,
-    nextBitCirc := fun a =>
-      match a with
-      | some () =>
-             -- If either succeeds, then the full thing succeeds
-             ((Circuit.var true (inr false)  &&&
-             ((Circuit.var false (inr true)) |||
-             -- On the other hand, if we have failed, then propagate failure.
-              (Circuit.var true (inl ())))))
-      | none => -- can succeed in either argument, so we are `0` if either is `0`.
-                Circuit.var true (inr true) &&&
-                Circuit.var true (inr false)
-                }
-
-/-- An `FSMPredicateSolution `t` is an FSM with a witness that the FSM evaluates to the same value as `t` does -/
-structure FSMPredicateSolution (p : Predicate) extends FSM (Fin p.arity) where
-  ( good : p.evalFin = toFSM.eval )
-
-
-
-/-- Evaluating the eq predicate equals the FSM value.
-
-Note that **this is the value that is run by decide**.
-
--/
-def predicateEvalEqFSM : ∀ (p : Predicate), FSMPredicateSolution p
-  | .widthEq n =>
-    {
-      toFSM := FSM.falseOnlyAt n
-      good := by sorry
-    }
-  | .widthNeq n =>
-     {
-      toFSM := FSM.trueOnlyAt n
-      good := by sorry
-     }
-  | .widthGe n =>
-     {
-      toFSM := FSM.falseAfterIncluding n
-      good := by sorry
-     }
-  | .widthGt n =>
-     {
-      toFSM := FSM.falseAfterExcluding n
-      good := by sorry
-     }
-  | .widthLt n =>
-     {
-      toFSM := FSM.falseUptoExcluding n
-      good := by sorry
-     }
-  | .widthLe n =>
-     {
-      toFSM := FSM.falseUptoIncluding n
-      good := by sorry
-     }
-  | .eq t₁ t₂ =>
-    let t₁' := termEvalEqFSM t₁
-    let t₂' := termEvalEqFSM t₂
-    {
-     toFSM := (composeBinary FSM.xor t₁' t₂')
-     good := by ext; simp;
-    }
-  | .neq t₁ t₂ =>
-    let t₁' := termEvalEqFSM t₁
-    let t₂' := termEvalEqFSM t₂
-    {
-     -- If it ever becomes `0`, it should stay `0` forever, because once
-     -- two bitstreams become disequal, they stay disequal!
-     toFSM := composeUnaryAux FSM.scanAnd <| (composeBinary FSM.nxor t₁' t₂')
-     good := by sorry -- ext; simp;
-    }
-   | .land p q =>
-     let x₁ := predicateEvalEqFSM p
-     let x₂ :=  predicateEvalEqFSM q
-     {
-       -- If this ever becomes `1`, it should stay `1`,
-       -- since once it's falsified, it should stay falsified!
-       toFSM := composeBinaryAux FSM.or x₁.toFSM x₂.toFSM
-       good := by sorry -- ext; simp [x₁.good, x₂.good]
-     }
-   | .lor p q =>
-     let x₁ := predicateEvalEqFSM p
-     let x₂ :=  predicateEvalEqFSM q
-     {
-       -- If it ever becomes `1`, it should stay `1`,
-       -- since one it's falsified, it should stay falsified!
-       toFSM := composeBinaryAux FSM.and x₁.toFSM x₂.toFSM
-       good := by sorry -- ext; simp [x₁.good, x₂.good]
-     }
-   | .slt t₁ t₂ =>
-     let q₁ := termEvalEqFSM t₁
-     let q₂ := termEvalEqFSM t₂
-     { toFSM := composeUnaryAux FSM.not <| composeBinary FSM.sub q₁ q₂,
-       good := by sorry --   ext; simp }
-     }
-   | .sle t₁ t₂ =>
-      let t₁' := termEvalEqFSM t₁
-      let t₂' := termEvalEqFSM t₂
-      let slt := (composeUnaryAux FSM.not <| composeBinaryAux FSM.sub t₁'.toFSM t₂'.toFSM)
-      let eq := (composeBinaryAux FSM.xor t₁'.toFSM t₂'.toFSM)
-      have hsz : max (max t₁.arity t₂.arity) (max t₁.arity t₂.arity) = (max t₁.arity t₂.arity) :=
-        Nat.max_self ..
-      have hsz : max (max t₁.arity t₂.arity) (max t₁.arity t₂.arity) = Predicate.arity (.sle t₁ t₂) := by
-        simp [hsz]
-      -- We want an OR of the two cases, which we take by computing an AND of the predicates.
-      let out := composeBinaryAux FSM.and slt eq
-      {
-       toFSM := hsz ▸ out
-       good := by sorry -- TODO: show that it's good 'ext; simp';
-      }
-   | .ult t₁ t₂ =>
-      let t₁' := termEvalEqFSM t₁
-      let t₂' := termEvalEqFSM t₂
-      {
-       -- a <u b if when we compute (a - b), we must borrow a value.
-       toFSM := (composeUnaryAux FSM.not $ composeBinary FSM.borrow t₁' t₂')
-       good := by sorry -- TODO: show that it's good 'ext; simp';
-      }
-   | .ule t₁ t₂ =>
-      let t₁' := termEvalEqFSM t₁
-      let t₂' := termEvalEqFSM t₂
-      let ult := (composeUnaryAux FSM.not $ composeBinaryAux FSM.borrow t₁'.toFSM t₂'.toFSM)
-      let eq := (composeBinaryAux FSM.xor t₁'.toFSM t₂'.toFSM)
-      have hsz : max (max t₁.arity t₂.arity) (max t₁.arity t₂.arity) = (max t₁.arity t₂.arity) :=
-        Nat.max_self ..
-      have hsz : max (max t₁.arity t₂.arity) (max t₁.arity t₂.arity) = Predicate.arity (.ule t₁ t₂) := by
-        simp [hsz]
-      -- IF either a < b, or a = b, then we know that a ≤ b.
-      let out := composeBinaryAux FSM.and ult eq
-      {
-       toFSM := hsz ▸ out
-       good := by sorry -- TODO: show that it's good 'ext; simp';
-      }
-
-def card_compl [Fintype α] [DecidableEq α] (c : Circuit α) : ℕ :=
-  Finset.card $ (@Finset.univ (α → Bool) _).filter (fun a => c.eval a = false)
-
-theorem decideIfZeroAux_wf {α : Type _} [Fintype α] [DecidableEq α]
-    {c c' : Circuit α} (h : ¬c' ≤ c) : card_compl (c' ||| c) < card_compl c := by
-  apply Finset.card_lt_card
-  simp [Finset.ssubset_iff, Finset.subset_iff]
-  simp only [Circuit.le_def, not_forall, Bool.not_eq_true] at h
-  rcases h with ⟨x, hx, h⟩
-  use x
-  simp [hx, h]
-
-def decideIfZerosAux {arity : Type _} [DecidableEq arity]
-    (p : FSM arity) (c : Circuit p.α) : Bool :=
-  if c.eval p.initCarry
-  then false
-  else
-    have c' := (c.bind (p.nextBitCirc ∘ some)).fst
-    if h : c' ≤ c then true
-    else
-      have _wf : card_compl (c' ||| c) < card_compl c :=
-        decideIfZeroAux_wf h
-      decideIfZerosAux p (c' ||| c)
-  termination_by card_compl c
-
-def decideIfZeros {arity : Type _} [DecidableEq arity]
-    (p : FSM arity) : Bool :=
-  decideIfZerosAux p (p.nextBitCirc none).fst
-
-theorem decideIfZerosAux_correct {arity : Type _} [DecidableEq arity]
-    (p : FSM arity) (c : Circuit p.α)
-    (hc : ∀ s, c.eval s = true →
-      ∃ m y, (p.changeInitCarry s).eval y m = true)
-    (hc₂ : ∀ (x : arity → Bool) (s : p.α → Bool),
-      (FSM.nextBit p s x).snd = true → Circuit.eval c s = true) :
-    decideIfZerosAux p c = true ↔ ∀ n x, p.eval x n = false := by
-  rw [decideIfZerosAux]
-  split_ifs with h
-  · simp
-    exact hc p.initCarry h
-  · dsimp
-    split_ifs with h'
-    · simp only [true_iff]
-      intro n x
-      rw [p.eval_eq_zero_of_set {x | c.eval x = true}]
-      · intro y s
-        simp [Circuit.le_def, Circuit.eval_fst, Circuit.eval_bind] at h'
-        simp [Circuit.eval_fst, FSM.nextBit]
-        apply h'
-      · assumption
-      · exact hc₂
-    · let c' := (c.bind (p.nextBitCirc ∘ some)).fst
-      have _wf : card_compl (c' ||| c) < card_compl c :=
-        decideIfZeroAux_wf h'
-      apply decideIfZerosAux_correct p (c' ||| c)
-      simp [c', Circuit.eval_fst, Circuit.eval_bind]
-      intro s hs
-      rcases hs with ⟨x, hx⟩ | h
-      · rcases hc _ hx with ⟨m, y, hmy⟩
-        use (m+1)
-        use fun a i => Nat.casesOn i x (fun i a => y a i) a
-        rw [FSM.eval_changeInitCarry_succ]
-        rw [← hmy]
-        simp only [FSM.nextBit, Nat.rec_zero, Nat.rec_add_one]
-      · exact hc _ h
-      · intro x s h
-        have := hc₂ _ _ h
-        simp only [Circuit.eval_bind, Bool.or_eq_true, Circuit.eval_fst,
-          Circuit.eval_or, this, or_true]
-termination_by card_compl c
-
-theorem decideIfZeros_correct {arity : Type _} [DecidableEq arity]
-    (p : FSM arity) : decideIfZeros p = true ↔ ∀ n x, p.simplify.eval x n = false := by
-  simp only [FSM.eval_simplify]
-  apply decideIfZerosAux_correct
-  · simp only [Circuit.eval_fst, forall_exists_index]
-    intro s x h
-    use 0
-    use (fun a _ => x a)
-    simpa [FSM.eval, FSM.changeInitCarry, FSM.nextBit, FSM.carry]
-  · simp only [Circuit.eval_fst]
-    intro x s h
-    use x
-    exact h
-
-/-- Iterate the next bit circuit 'n' times, while universally quantifying over all inputs
-that are possible at each step. -/
-def FSM.nextBitCircIterate {arity : Type _ } [DecidableEq arity]
-    (fsm : FSM arity) (n : Nat) : Circuit fsm.α :=
-  match n with
-  | 0 => fsm.nextBitCirc none |>.fst
-  | n' + 1 =>
-     -- | the .fst performs quantifier elimination, by running over all possible values of inputs.
-     let c := fsm.nextBitCircIterate n'
-     (c.bind (fsm.nextBitCirc ∘ some)).fst
-
-/-- Decide if the FSM produces zeroes for all inputs at a given index of the bitstream -/
-def decideIfZerosAtIx {arity : Type _} [DecidableEq arity]
-      (fsm : FSM arity) (w : Nat) : Bool :=
-    let c := fsm.nextBitCircIterate w
-    c.eval fsm.initCarry
-
-/--
-The correctness statement of 'denoteIfZeroesAtIx'.
-This tells us that 'denoteIfZeroesAtIx' is correct iff the FSM 'p' when evaluated returns false
-for all inputs at the index 'w' of the bitstream
--/
-theorem decideIfZeroesAtIx_correct {arity : Type _} [DecidableEq arity]
-    (p : FSM arity) (w : Nat) : decideIfZerosAtIx p w = true ↔ ∀ x, p.eval x w = false := by
-  sorry
+abbrev FSM.ofTerm (t : Term) : FSM (Fin t.arity) := termEvalEqFSM t |>.toFSM
 
 end FSM
